src/compiler/meta/OCL_compiler_parser_UML.thy
@@ -79,8 +79,7 @@ definition "ocl_ty_class_rec f ocl = ocl_ty_class_rec0 f ocl
 definition "ocl_class_raw_rec0 f ocl = f
   (ClassRaw_name ocl)
   (ClassRaw_own ocl)
-  (ClassRaw_contract ocl)
-  (ClassRaw_invariant ocl)
+  (ClassRaw_clause ocl)
   (ClassRaw_abstract ocl)"
 
 definition "ocl_class_raw_rec f ocl = ocl_class_raw_rec0 f ocl
@@ -94,38 +93,36 @@ definition "ocl_association_rec f ocl = ocl_association_rec0 f ocl
   (ocl_association.more ocl)"
 
 definition "ocl_ctxt_pre_post_rec0 f ocl = f
-  (Ctxt_ty ocl)
   (Ctxt_fun_name ocl)
-  (Ctxt_fun_ty_arg ocl)
-  (Ctxt_fun_ty_out ocl)
+  (Ctxt_fun_ty ocl)
   (Ctxt_expr ocl)"
 
 definition "ocl_ctxt_pre_post_rec f ocl = ocl_ctxt_pre_post_rec0 f ocl
   (ocl_ctxt_pre_post.more ocl)"
 
-definition "ocl_ctxt_inv_rec0 f ocl = f
-  (Ctxt_inv_param ocl)
-  (Ctxt_inv_ty ocl)
-  (Ctxt_inv_expr ocl)"
+definition "ocl_ctxt_rec0 f ocl = f
+  (Ctxt_param ocl)
+  (Ctxt_ty ocl)
+  (Ctxt_clause ocl)"
 
-definition "ocl_ctxt_inv_rec f ocl = ocl_ctxt_inv_rec0 f ocl
-  (ocl_ctxt_inv.more ocl)"
+definition "ocl_ctxt_rec f ocl = ocl_ctxt_rec0 f ocl
+  (ocl_ctxt.more ocl)"
 
 (* *)
 
-lemma [code]: "ocl_class_raw.extend = (\<lambda>ocl v. ocl_class_raw_rec0 (co5 (\<lambda>f. f v) ocl_class_raw_ext) ocl)"
+lemma [code]: "ocl_class_raw.extend = (\<lambda>ocl v. ocl_class_raw_rec0 (co4 (\<lambda>f. f v) ocl_class_raw_ext) ocl)"
 by(intro ext, simp add: ocl_class_raw_rec0_def
                         ocl_class_raw.extend_def
-                        co5_def K_def)
-lemma [code]: "ocl_class_raw.make = co5 (\<lambda>f. f ()) ocl_class_raw_ext"
+                        co4_def K_def)
+lemma [code]: "ocl_class_raw.make = co4 (\<lambda>f. f ()) ocl_class_raw_ext"
 by(intro ext, simp add: ocl_class_raw.make_def
-                        co5_def)
-lemma [code]: "ocl_class_raw.truncate = ocl_class_raw_rec (co5 K ocl_class_raw.make)"
+                        co4_def)
+lemma [code]: "ocl_class_raw.truncate = ocl_class_raw_rec (co4 K ocl_class_raw.make)"
 by(intro ext, simp add: ocl_class_raw_rec0_def
                         ocl_class_raw_rec_def
                         ocl_class_raw.truncate_def
                         ocl_class_raw.make_def
-                        co5_def K_def)
+                        co4_def K_def)
 
 lemma [code]: "ocl_association.extend = (\<lambda>ocl v. ocl_association_rec0 (co2 (\<lambda>f. f v) ocl_association_ext) ocl)"
 by(intro ext, simp add: ocl_association_rec0_def
@@ -187,10 +184,10 @@ definition "i_of_ocl_ty_obj_core a b = rec_ocl_ty_obj_core
 definition "i_of_ocl_ty_obj a b = rec_ocl_ty_obj
   (ap2 a (b \<open>OclTyObj\<close>) (i_of_ocl_ty_obj_core a b) (i_of_list a b (i_of_list a b (i_of_ocl_ty_obj_core a b))))"
 
-definition "i_of_ocl_ty a b = (\<lambda>f1 f2 f3 f4 f5 f6 f7 f8 f9 f10 f11 f12 f13 f14 f15.
+definition "i_of_ocl_ty a b = (\<lambda>f1 f2 f3 f4 f5 f6 f7 f8 f9 f10 f11 f12 f13.
                                     rec_ocl_ty_1 f1 f2 f3 f4 f5 f6
                                                  f7 (K o f8) (\<lambda>_ _. f9) (\<lambda>_. f10) (\<lambda>_ _. f11) f12
-                                                 (K o f13) (K o f14) (K o f15))
+                                                 (K o f13))
   (b \<open>OclTy_base_void\<close>)
   (b \<open>OclTy_base_boolean\<close>)
   (b \<open>OclTy_base_integer\<close>)
@@ -200,12 +197,10 @@ definition "i_of_ocl_ty a b = (\<lambda>f1 f2 f3 f4 f5 f6 f7 f8 f9 f10 f11 f12 f
   (ap1 a (b \<open>OclTy_object\<close>) (i_of_ocl_ty_obj a b))
   (ar2 a (b \<open>OclTy_collection\<close>) (i_of_ocl_multiplicity a b (K i_of_unit)))
   (ar2 a (b \<open>OclTy_pair\<close>) id)
-  (ar1 a (b \<open>OclTy_pair1\<close>))
+  (ar1 a (b \<open>OclTy_binding\<close>))
   (ar2 a (b \<open>OclTy_arrow\<close>) id)
   (ap1 a (b \<open>OclTy_raw\<close>) (i_of_string a b))
   (* *)
-  (curry (i_of_pair a b (i_of_option a b (i_of_string a b)) id))
-  (curry (i_of_pair a b (i_of_option a b (i_of_string a b)) id))
   (curry (i_of_pair a b (i_of_option a b (i_of_string a b)) id))"
 
 definition "i_of_ocl_association_type a b = rec_ocl_association_type
@@ -214,10 +209,14 @@ definition "i_of_ocl_association_type a b = rec_ocl_association_type
   (b \<open>OclAssTy_composition\<close>)
   (b \<open>OclAssTy_aggregation\<close>)"
 
+definition "i_of_ocl_association_relation a b = rec_ocl_association_relation
+  (ap1 a (b \<open>OclAssRel\<close>)
+    (i_of_list a b (i_of_pair a b (i_of_ocl_ty_obj a b) (i_of_ocl_multiplicity a b (K i_of_unit)))))"
+
 definition "i_of_ocl_association a b f = ocl_association_rec
   (ap3 a (b (ext \<open>ocl_association_ext\<close>))
     (i_of_ocl_association_type a b)
-    (i_of_list a b (i_of_pair a b (i_of_ocl_ty_obj a b) (i_of_ocl_multiplicity a b (K i_of_unit))))
+    (i_of_ocl_association_relation a b)
     (f a b))"
 
 definition "i_of_ocl_ctxt_prefix a b = rec_ocl_ctxt_prefix
@@ -229,20 +228,32 @@ definition "i_of_ocl_ctxt_term a b = (\<lambda>f0 f1 f2. rec_ocl_ctxt_term f0 f1
   (ap2 a (b \<open>T_to_be_parsed\<close>) (i_of_string a b) (i_of_string a b))
   (ar2 a (b \<open>T_lambda\<close>) (i_of_string a b))"
 
+definition "i_of_ocl_prop a b = rec_ocl_prop
+  (ap2 a (b \<open>OclProp_ctxt\<close>) (i_of_option a b (i_of_string a b)) (i_of_ocl_ctxt_term a b))"
+
+definition "i_of_ocl_ctxt_term_inv a b = rec_ocl_ctxt_term_inv
+  (ap2 a (b \<open>T_inv\<close>) (i_of_bool b) (i_of_ocl_prop a b))"
+
+definition "i_of_ocl_ctxt_term_pp a b = rec_ocl_ctxt_term_pp
+  (ap2 a (b \<open>T_pp\<close>) (i_of_ocl_ctxt_prefix a b) (i_of_ocl_prop a b))
+  (ap1 a (b \<open>T_invariant\<close>) (i_of_ocl_ctxt_term_inv a b))"
+
 definition "i_of_ocl_ctxt_pre_post a b f = ocl_ctxt_pre_post_rec
-  (ap6 a (b (ext \<open>ocl_ctxt_pre_post_ext\<close>))
+  (ap4 a (b (ext \<open>ocl_ctxt_pre_post_ext\<close>))
     (i_of_string a b)
-    (i_of_string a b)
-    (i_of_list a b (i_of_pair a b (i_of_string a b) (i_of_ocl_ty a b)))
-    (i_of_option a b (i_of_ocl_ty a b))
-    (i_of_list a b (i_of_pair a b (i_of_ocl_ctxt_prefix a b) (i_of_ocl_ctxt_term a b)))
+    (i_of_ocl_ty a b)
+    (i_of_list a b (i_of_ocl_ctxt_term_pp a b))
     (f a b))"
 
-definition "i_of_ocl_ctxt_inv a b f = ocl_ctxt_inv_rec
-  (ap4 a (b (ext \<open>ocl_ctxt_inv_ext\<close>))
+definition "i_of_ocl_ctxt_clause a b = rec_ocl_ctxt_clause
+  (ap1 a (b \<open>Ctxt_pp\<close>) (i_of_ocl_ctxt_pre_post a b (K i_of_unit)))
+  (ap1 a (b \<open>Ctxt_inv\<close>) (i_of_ocl_ctxt_term_inv a b))"
+
+definition "i_of_ocl_ctxt a b f = ocl_ctxt_rec
+  (ap4 a (b (ext \<open>ocl_ctxt_ext\<close>))
     (i_of_list a b (i_of_string a b))
-    (i_of_string a b)
-    (i_of_list a b (i_of_pair a b (i_of_string a b) (i_of_ocl_ctxt_term a b)))
+    (i_of_ocl_ty_obj a b)
+    (i_of_list a b (i_of_ocl_ctxt_clause a b))
     (f a b))"
 
 definition "i_of_ocl_class a b = (\<lambda>f0 f1 f2 f3 f4. rec_ocl_class_1 (co2 K (ar3 a f0 f1 f2)) f3 (\<lambda>_ _. f4))
@@ -254,11 +265,10 @@ definition "i_of_ocl_class a b = (\<lambda>f0 f1 f2 f3 f4. rec_ocl_class_1 (co2 
     (ar2 a (b i_Cons) id)"
 
 definition "i_of_ocl_class_raw a b f = ocl_class_raw_rec
-  (ap6 a (b (ext \<open>ocl_class_raw_ext\<close>))
+  (ap5 a (b (ext \<open>ocl_class_raw_ext\<close>))
     (i_of_ocl_ty_obj a b)
     (i_of_list a b (i_of_pair a b (i_of_string a b) (i_of_ocl_ty a b)))
-    (i_of_list a b (i_of_ocl_ctxt_pre_post a b (K i_of_unit)))
-    (i_of_list a b (i_of_ocl_ctxt_inv a b (K i_of_unit)))
+    (i_of_list a b (i_of_ocl_ctxt_clause a b))
     (i_of_bool b)
     (f a b))"
 
@@ -279,11 +289,16 @@ lemmas [code] =
   i_of.i_of_ocl_ty_obj_def
   i_of.i_of_ocl_ty_def
   i_of.i_of_ocl_association_type_def
+  i_of.i_of_ocl_association_relation_def
   i_of.i_of_ocl_association_def
   i_of.i_of_ocl_ctxt_prefix_def
   i_of.i_of_ocl_ctxt_term_def
+  i_of.i_of_ocl_prop_def
+  i_of.i_of_ocl_ctxt_term_inv_def
+  i_of.i_of_ocl_ctxt_term_pp_def
   i_of.i_of_ocl_ctxt_pre_post_def
-  i_of.i_of_ocl_ctxt_inv_def
+  i_of.i_of_ocl_ctxt_clause_def
+  i_of.i_of_ocl_ctxt_def
   i_of.i_of_ocl_class_def
   i_of.i_of_ocl_class_raw_def
   i_of.i_of_ocl_ass_class_def
